init_l2ptable verifies!
This necessitated some minor refactoring of the relevant pagedb and
smcapi defs, to reuse portions of the spec in the impl proof. I also
backed out the "optimisation" to avoid the early check for a stopped
addrspace... saving a load and conditional branch is not worth the
hours of verification time this was going to take!

verified/pagedb.s.dfy
@@ -6,7 +6,7 @@ include "ARMdef.dfy"
 type PageNr = int
 type InsecurePageNr = int
 
-function NR_L1PTES(): int { 256 }
+function method NR_L1PTES(): int { 256 }
 function NR_L2PTES(): int { 1024 }
 
 predicate validPageNr(p: PageNr)
